examples/scalaEquivalenceBenchmarkExamples/noHelp/intro.dfy
@@ -12,28 +12,28 @@ function insertM(xs: List<int>, t: int): List<int>
   }
 }
 
-function insertRandomSortedM<Seed>(seed: Seed, next: Seed -> (Seed, int), count: int, xs: List<int>): List<int>
+function insertSortedM<Seed>(seed: Seed, next: Seed -> (Seed, int), count: int, xs: List<int>): List<int>
   {
   if (count <= 0) then xs
   else
     var (nxtS, t) := next(seed);
-    insertRandomSortedM(nxtS, next, count - 1, insertM(xs, t))
+    insertSortedM(nxtS, next, count - 1, insertM(xs, t))
 }
 
 function insert1(t: int, xs: List<int>): List<int>
   decreases xs {
   match xs {
-    case Nil => Cons(t, Nil)
     case Cons(hd, tl) =>
-      if (t <= hd) then Cons(t, xs)
-      else Cons(hd, insert1(t, tl))
+      if (!(t <= hd)) then Cons(hd, insert1(t, tl))
+      else Cons(t, xs)
+    case Nil => Cons(t, Nil)
   }
 }
 
-function insertRandomSorted1<Seed>(seed: Seed, next: Seed -> (Seed, int), xs: List<int>, count: int): List<int>
+function insertSorted1<Seed>(seed: Seed, next: Seed -> (Seed, int), xs: List<int>, count: int): List<int>
   decreases count {
-  if (count <= 0) then xs
-  else
+  if (!(count <= 0)) then 
     var (nxtS, t) := next(seed);
-    insertRandomSorted1(nxtS, next, insert1(t, xs), count - 1)
+    insertSorted1(nxtS, next, insert1(t, xs), count - 1)
+  else xs
 }
